body_kalloc_write_42, body_kfree_kalloc and impl is almost verified

kalloc/kallocfun.v
@@ -17,10 +17,14 @@ Definition t_run_size := sizeof t_run.
 (* ================================================================= *)
 (** ** Size-based kalloc tokens *)
 
+Definition forall_small_PGSIZE p : Prop :=
+  (forall n : Z, (0 < n <= PGSIZE /\ ((isptr p /\ 0 < n <= PGSIZE /\ malloc_compatible (n) p)))).
+  (*ALL n : Z, !! (0 < n <= PGSIZE /\ ((isptr p /\ 0 < n <= PGSIZE /\ malloc_compatible (n) p) \/ (p = nullval))).*)
+
 Definition kalloc_token_sz (sh: share) (n: Z) (p: val) : mpred :=
   !! (
       0 < n <= PGSIZE 
-      /\ malloc_compatible n p
+      /\ forall_small_PGSIZE p
       /\ writable_share sh
       /\ field_compatible t_run [] p (* make sure t_run fits*)
       /\ malloc_compatible (sizeof t_run) p 
@@ -30,14 +34,16 @@ Definition kalloc_token_sz (sh: share) (n: Z) (p: val) : mpred :=
          | _ => True
          end
       (*/\  maybe some alignment and physical address checks here *))
-  && memory_block sh PGSIZE (p).
+  && ((*sepcon (forall_small_PGSIZE p) *)
+  (sepcon (memory_block sh (t_run_size) (p)) (memory_block sh (PGSIZE - t_run_size)
+  (offset_val t_run_size p))) ).
 
 Lemma kalloc_token_sz_valid_pointer:
   forall (sh : share) (sz : Z) (p : val),
   kalloc_token_sz sh sz p |-- valid_pointer p.
 Proof.
   intros. 
-  unfold kalloc_token_sz. entailer.
+  unfold kalloc_token_sz. unfold t_run_size. entailer.
 Qed.
 
 Lemma  kalloc_token_sz_local_facts : 
@@ -45,7 +51,10 @@ Lemma  kalloc_token_sz_local_facts :
    kalloc_token_sz sh n p |-- !! malloc_compatible n p.
 Proof.
   intros. 
-  unfold kalloc_token_sz. simpl. entailer.
+  unfold kalloc_token_sz. Intros. entailer. unfold forall_small_PGSIZE in H0.
+  specialize (H0 n). entailer!.
+  destruct H0 as [HH0 [HH1 [HH2 HH3]]].
+  auto. 
 Qed.
 
 Lemma kalloc_token_sz_split:
@@ -53,39 +62,72 @@ forall  (sh: share) (n: Z) (p: val),
   kalloc_token_sz sh n p =
   !! (
       0 < n <= PGSIZE 
-      /\ malloc_compatible n p 
+      /\ forall_small_PGSIZE p
       /\ writable_share sh
       /\ field_compatible t_run [] p (* make sure t_run fits*)
       /\ malloc_compatible (sizeof t_run) p 
       /\ 0 < (sizeof t_run) <= PGSIZE 
       /\ match p with
          | Vptr _ ofs => Ptrofs.unsigned ofs + PGSIZE < Ptrofs.modulus
-         | _ => True (* this is not important if the p is not a pointer *)
+         | _ => True
          end
       (*/\  maybe some alignment and physical address checks here *))
-  && memory_block sh PGSIZE (p).
+  && ((*sepcon (forall_small_PGSIZE p) *)
+  (sepcon (memory_block sh (t_run_size) (p)) (memory_block sh (PGSIZE - t_run_size)
+  (offset_val t_run_size p))) ).
 Proof.
   intros. apply pred_ext.
   - unfold kalloc_token_sz. entailer.
   - unfold kalloc_token_sz. entailer!.
 Qed.
 
+Lemma token_merge :
+forall (sh: share) (p:val) b i,
+isptr p ->
+p = Vptr b i ->
+PGSIZE + Ptrofs.unsigned i < Ptrofs.modulus ->
+(sepcon (memory_block sh t_run_size p)
+  (memory_block sh (PGSIZE - t_run_size) (offset_val t_run_size p)) 
+  = memory_block sh PGSIZE p
+  ).
+Proof.
+destruct p; auto_contradict.
+assert (i = Ptrofs.repr (Ptrofs.unsigned i)) as HH. { rewrite Ptrofs.repr_unsigned. auto. }
+unfold offset_val. rewrite Ptrofs.add_unsigned.
+rewrite Ptrofs.unsigned_repr.
+intros.
+rewrite HH at 1.
+rewrite <- memory_block_split.
+assert (t_run_size + (PGSIZE - t_run_size) = PGSIZE) as Hpgsz; try rep_lia.
+rewrite Hpgsz. rewrite HH at 2. auto.
+- unfold t_run_size. simpl; try rep_lia.
+- unfold t_run_size. simpl; try rep_lia.
+- unfold t_run_size. simpl; try rep_lia. split; try rep_lia.
+inversion H0. unfold PGSIZE in H1; auto.
+- unfold t_run_size. simpl; try rep_lia.
+Qed.
+
 
 (* ================================================================= *)
 (** ** Defining freelistrep *)
+
 
 (* NOTE: assume PGSIZE is greater than sizeof t_run *)
 Fixpoint freelistrep (sh: share) (il: list val) (p: val) : mpred := (* the list contains the next*)
  match il with
  | next::il' =>
-        !!(malloc_compatible (sizeof t_run) p 
+        (!!(malloc_compatible (sizeof t_run) p 
           /\ match p with
           | Vptr _ ofs => Ptrofs.unsigned ofs + PGSIZE < Ptrofs.modulus
           | _ => True
           end
+          /\
+          forall_small_PGSIZE p
           ) &&  (* p is compatible with a memory block of size sizeof theader. *)
-          (sepcon (data_at sh t_run next p) (* at the location p, there is a t_run structure with the value next *)
-          (freelistrep sh il' next) (* "*" ensures no loops... *))
+          (
+          (sepcon (sepcon (data_at sh t_run next p) 
+                    (memory_block sh (PGSIZE - t_run_size) (offset_val t_run_size p))) (* at the location p, there is a t_run structure with the value next *)
+          (freelistrep sh il' next) (* "*" ensures no loops... *))))
  | nil => !! (p = nullval) && emp
  end.
 
@@ -100,7 +142,7 @@ Proof.
     + split; auto.
     + split; try lia. intros. simpl in *. auto_contradict. intros; auto_contradict.
   - unfold freelistrep. fold freelistrep. destruct p; entailer!. split.
-    + split; intros; inversion H3.
+    + split; intros; inversion H5.
     + split; intros; auto. unfold not; intros. auto_contradict.
    Qed.
 #[export] Hint Resolve freelistrep_local_prop : saturate_local.
