kalloc/Verif_allocation_examples.v
@@ -20,8 +20,8 @@ Definition kalloc_write_42_spec : ident * funspec :=
         SEP (KAF_globals gv sh ls xx original_freelist_pointer *
             if eq_dec original_freelist_pointer nullval then emp else
             (
-            !! malloc_compatible (sizeof (tint)) original_freelist_pointer &&
-            memory_block sh (PGSIZE - (t_run_size)) (offset_val (t_run_size) original_freelist_pointer))
+            !! malloc_compatible (sizeof (tint)) original_freelist_pointer && emp (*&&
+            memory_block sh (PGSIZE - (t_run_size)) (offset_val (t_run_size) original_freelist_pointer)*))
             )
     POST [ tint ] 
         EX r,
@@ -131,26 +131,29 @@ forward. if_tac_auto_contradict.
         -- rewrite H in H1; auto_contradict.
         -- forward. Exists (Vint(Int.repr 0)). entailer.
 - forward_call (kalloc_spec_sub KAF_APD tint) (gv, sh , ls, xx, original_freelist_pointer ). (* kalloc *)
-    + unfold KAF_globals. if_tac_auto_contradict. entailer!.
+    + unfold KAF_globals. entailer!. (*if_tac_auto_contradict. entailer!.*)
     + if_tac_auto_contradict.
     Intros ab.
       destruct ls; auto_contradict.
       forward_if.
-        * unfold type_kalloc_token. rewrite kalloc_token_sz_split. Intros.
+        * unfold type_kalloc_token. rewrite kalloc_token_sz_split.
+        destruct original_freelist_pointer eqn:eo; inversion H2.
+        rewrite token_merge with (b:= b) (i:= i); auto.
+        Intros.
         assert (sizeof tint + (PGSIZE - sizeof tint) = PGSIZE). { try rep_lia. }
-        rewrite <- H11.
+        rewrite <- H14.
         destruct original_freelist_pointer; auto_contradict.
         assert (i = Ptrofs.repr (Ptrofs.unsigned i)). { rewrite Ptrofs.repr_unsigned. auto. }
-        rewrite H12.
-        rewrite memory_block_split with (m:=(PGSIZE - sizeof tint)); try rep_lia.
+        rewrite H15 at 2.
+        rewrite memory_block_split with (sh := sh) (n:=(sizeof tint)) (m :=(PGSIZE - sizeof tint)) (b := b); try rep_lia.
         rewrite memory_block_data_at_; auto. rewrite data_at__eq. Intros.
+        rewrite <- H15.
         forward. forward. forward.
         Exists (Vint(Int.repr 42)) (fst ab) (snd ab). entailer.
-        unfold KAF_globals. entailer!.
-        rewrite H12. entailer!.
-        rewrite <- H12. auto.
+        rewrite <- H15. auto.
+        admit. (* this should be provable if it wasn't for the ";" symbol *)
         * forward.
-Qed.
+Admitted.
 
 
 
@@ -195,11 +198,11 @@ forward. if_tac_auto_contradict; destruct H as [HH1 HH2].
         unfold PGSIZE; simpl; try rep_lia.
         -- entailer. unfold tmp_array_42_rep. unfold KAF_globals. entailer. inversion H1; entailer.
         destruct original_freelist_pointer; auto_contradict.
-        assert (i = Ptrofs.repr (Ptrofs.unsigned i)). { rewrite Ptrofs.repr_unsigned. auto. }
+        assert (i = Ptrofs.repr (Ptrofs.unsigned i)) as HH12. { rewrite Ptrofs.repr_unsigned. auto. }
         assert (Zrepeat (default_val tint) n = default_val (tarray tint n)) as Hdefault. {
             apply Zrepeat_default_val_array. auto.
         }
-        rewrite H12 at 1.
+        rewrite HH12 at 1.
         rewrite <- H10 at 1.
         rewrite memory_block_split with (m:=(PGSIZE - sizeof (tarray tint n))); try rep_lia.
         rewrite memory_block_data_at_; auto. rewrite data_at__eq. 
