kalloc/Verif_kalloc_kfree.v
@@ -11,6 +11,7 @@ Require Import VC.Spec_kalloc.
 
 Local Open Scope logic.
 
+
 (*Lemma body_kfree: semax_body KAFVprog KAFGprog f_kfree (kfree_spec KAF_APD t_run).
 Proof. start_function. Intros.
 forward.
@@ -37,26 +38,26 @@ destruct (eq_dec new_head nullval).
     * rewrite e in H2; auto_contradict.
     * forward. entailer. rewrite mem_mgr_split. entailer.
 - forward_if.
-    * forward. rewrite kalloc_token_sz_split. Intros. 
+    * Intros. forward. rewrite kalloc_token_sz_split. Intros. 
     assert (memory_block sh ((sizeof t_run) + (PGSIZE-sizeof t_run)) new_head = memory_block sh PGSIZE new_head).
     {
         simpl. unfold PGSIZE. auto.
     }
-    rewrite <- H9.
-    destruct new_head; auto_contradict.
+    (*rewrite <- H9.*)
+    (*destruct new_head; auto_contradict.
     assert (memory_block sh ((sizeof t_run) + (PGSIZE - sizeof t_run)) (Vptr b i) = memory_block sh ((sizeof t_run) + (PGSIZE - sizeof t_run)) (Vptr b (Ptrofs.repr (Ptrofs.unsigned i)))). {
         simpl. rewrite Ptrofs.repr_unsigned. auto.
-    }
-    rewrite H10.
-    rewrite memory_block_split; try rep_lia.
+    }*)
+    (*rewrite H10.*)
+    (*rewrite memory_block_split; try rep_lia.
     assert (Vptr b (Ptrofs.repr (Ptrofs.unsigned i)) = Vptr b (i)). { rewrite Ptrofs.repr_unsigned. auto. }
-    rewrite memory_block_data_at_.
+    *) unfold t_run_size. rewrite memory_block_data_at_.
     Intros.
-    rewrite data_at__eq. rewrite H11. forward. forward. 
+    rewrite data_at__eq. (*rewrite H11.*) forward. forward. 
     entailer. rewrite mem_mgr_split. refold_freelistrep. entailer!.
-    right; split; auto. unfold not; auto_contradict. 
-    unfold t_run_size. unfold offset_val. rewrite Ptrofs.add_unsigned. rewrite Ptrofs.unsigned_repr.
-    entailer!. simpl. try rep_lia. rewrite H11. auto.
+    right; split; auto. unfold not; auto_contradict.
+    unfold t_run_size. unfold forall_small_PGSIZE. entailer!.
+    auto.
     * forward. entailer.
 Qed.
 
@@ -64,8 +65,6 @@ Qed.
 Lemma body_kalloc: semax_body KAFVprog KAFGprog f_kalloc (kalloc_spec' (KAF_APD) _kalloc).
 Proof. start_function.
 rewrite mem_mgr_split. Intros. forward. 
-if_tac.
--
 forward_if (
     PROP  ( )
     LOCAL (
@@ -85,11 +84,33 @@ forward_if (
         )
     )
 )%assert.
+- destruct H1 as [[H0011 H0012] | [H0021 H0022]].
++ rewrite H0012 in H2; auto_contradict.
++ destruct ls; auto_contradict.
+refold_freelistrep. Intros.
+forward. forward.
+entailer.
+rewrite mem_mgr_split. Intros. 
+refold_freelistrep. if_tac.
+* rewrite H13 in H0022; auto_contradict.
+* entailer. Exists v ls. entailer. 
+rewrite kalloc_token_sz_split. rewrite mem_mgr_split. entailer.
+unfold forall_small_PGSIZE. entailer!.
+-- destruct ls.
+    ++ left; split; auto. rewrite <- H11. auto.
+    ++ right. split.
+        **  unfold not. intros; auto_contradict.
+        ** rewrite <- H12. unfold not; intros; auto_contradict.
+-- apply data_at_memory_block.
+-forward. destruct (eq_dec original_freelist_pointer nullval) eqn:e1; auto_contradict. entailer.
+rewrite mem_mgr_split. entailer.
+- if_tac; forward.
+(*
 + rewrite H2 in H3. auto_contradict.
 + forward. if_tac; auto_contradict. entailer!.
     rewrite mem_mgr_split. entailer!.
 + if_tac_auto_contradict. forward.
--
+- (*unfold abbreviate in POSTCONDITION.*)
 forward_if (
     PROP  ( )
     LOCAL (
@@ -104,6 +125,7 @@ forward_if (
           EX next ls',
           (!! (next :: ls' = ls) &&
               kalloc_token' KAF_APD sh n original_freelist_pointer *
+              (*memory_block sh (PGSIZE - t_run_size) (offset_val t_run_size original_freelist_pointer) **)
               ASI_kalloc.mem_mgr KAF_APD gv sh ls' xx next
           )
         )
@@ -119,19 +141,19 @@ forward_if (
     rewrite mem_mgr_split. Intros. 
     refold_freelistrep. if_tac.
     -- rewrite H14 in H0022; auto_contradict.
-    -- entailer. Exists v ls. entailer. unfold type_kalloc_token.
+    -- entailer. Exists v ls. entailer.
     rewrite kalloc_token_sz_split. rewrite mem_mgr_split. entailer!.
     ++ destruct ls.
-     left; split; auto. rewrite <- H10; auto.
+     left; split; auto. rewrite <- H12; auto.
      right; split; auto. unfold not; intros. auto_contradict.
-     rewrite <- H11. unfold not; intros. auto_contradict.
+     rewrite <- H13. unfold not; intros. auto_contradict.
     ++ 
- 
     sep_apply data_at_memory_block. unfold offset_val. destruct original_freelist_pointer; auto_contradict. 
     assert (Ptrofs.add i (Ptrofs.repr t_run_size) = Ptrofs.repr (Ptrofs.unsigned i + t_run_size)). {
     rewrite Ptrofs.add_unsigned. rewrite Ptrofs.unsigned_repr; unfold t_run_size; simpl; try rep_lia. auto.
     }
-    rewrite H15.
+    unfold t_run_size. entailer.
+    (*rewrite H15.
     assert (i = Ptrofs.repr (Ptrofs.unsigned i)). { rewrite Ptrofs.repr_unsigned. auto. }
     replace (i) with (Ptrofs.repr (Ptrofs.unsigned i)) at 1.
     entailer!.
@@ -140,61 +162,17 @@ forward_if (
     **
     rewrite <- H16 at 1. 
     assert (t_run_size + (PGSIZE - t_run_size) = PGSIZE). { simpl. unfold PGSIZE; try rep_lia. }
-    rewrite H19. entailer!.
+    rewrite H19. entailer.
     ** 
     unfold t_run_size; simpl; try rep_lia.
     **
     unfold PGSIZE, t_run_size; simpl; try rep_lia.
-    ** simpl. split; try rep_lia. unfold PGSIZE in H4; try rep_lia.
+    ** simpl. split; try rep_lia. unfold PGSIZE in H4; try rep_lia.*)
     + forward. entailer.
     + forward. if_tac_auto_contradict. Intros next ls'.
     Exists next ls'. 
-    entailer!.
+    entailer!.*)
 Qed.
 
 
-
-(*Lemma body_kalloc: semax_body KAFVprog KAFGprog f_kalloc (kalloc_spec (KAF_APD) t_run).
-Proof. start_function.
-rewrite mem_mgr_split. Intros. forward.
-forward_if (
-    PROP  ( )
-    LOCAL (
-        temp _r original_freelist_pointer; 
-        gvars gv
-        )
-    SEP (
-        if (eq_dec original_freelist_pointer nullval) then
-        (ASI_kalloc.mem_mgr KAF_APD gv sh ls xx original_freelist_pointer * emp)
-      else 
-        (
-          EX next ls',
-          (!! (next :: ls' = ls) &&
-              type_kalloc_token KAF_APD sh (t_run) original_freelist_pointer *
-              ASI_kalloc.mem_mgr KAF_APD gv sh ls' xx next
-          )
-        )
-    )
-)%assert.
-- destruct H3 as [[H0011 H0012] | [H0021 H0022]].
-    + rewrite H0012 in H4; auto_contradict.
-    + destruct ls; auto_contradict.
-    refold_freelistrep. Intros.
-    forward. forward.
-    entailer.
-    rewrite mem_mgr_split. Intros. 
-    refold_freelistrep. if_tac.
-    * rewrite H11 in H0022; auto_contradict.
-    * entailer. Exists v ls. entailer. unfold type_kalloc_token.
-    rewrite kalloc_token_sz_split. rewrite mem_mgr_split. entailer!.
-    -- destruct ls.
-        ++ left; split; auto. rewrite <- H9; auto.
-        ++ right. split.
-            **  unfold not. intros; auto_contradict.
-            ** rewrite <- H10. unfold not; intros; auto_contradict.
-    -- apply data_at_memory_block.
--forward. destruct (eq_dec original_freelist_pointer nullval) eqn:e1; auto_contradict. entailer.
-rewrite mem_mgr_split. entailer.
-- if_tac; forward.
-Qed.*)
 
